RISC-V: add "select" operator
With a portable, inefficient implementation.

riscV/Asmexpand.ml
@@ -557,6 +557,25 @@ let expand_ctz ~sixtyfour ~splitlong =
                      else Psrliw(X6, X X6, coqint_of_camlint 31l));
   emit (Psubw(X7, X X7, X X6))
 
+(* Full register width "and", "xor" *)
+
+let _Pand (r, a1, a2) =
+  if Archi.ptr64 then Pandl(r, a1, a2) else Pandw(r, a1, a2)
+let _Pxor (r, a1, a2) =
+  if Archi.ptr64 then Pxorl(r, a1, a2) else Pxorw(r, a1, a2)
+
+(* Conditional move *)
+(* res <- if cond then arg1 else arg2
+   cond must be 0 or 1. *)
+
+let expand_csel res cond arg1 arg2 =
+  emit (Psubw(X31, X0, cond)); (* X31 = -1 if cond = 1, 0 if cond = 0 *)
+  emit (_Pxor(X1, arg1, arg2));
+  emit (_Pand(X1, X X1, X X31));
+  emit (_Pxor(res, arg2, X X1))
+     (* res = (arg1 ^ arg2) ^ arg2 = arg1  if cond = 1
+        res = 0 ^ arg2 = arg2              if cond = 0 *)
+
 (* Handling of compiler-inlined builtins *)
 
 let expand_builtin_inline name args res =
@@ -697,6 +716,8 @@ let expand_instruction instr =
       end else 0 in
      expand_addptrofs X2 X2 (Ptrofs.repr (Z.add sz (Z.of_uint extra_sz)))
 
+  | Pcsel(rd, rcond, rs1, rs2) ->
+      expand_csel rd (X rcond) (X rs1) (X rs2)
   | Pseqw(rd, rs1, rs2) ->
       (* emulate based on the fact that x == 0 iff x <u 1 (unsigned cmp) *)
       if rs2 = X0 then begin
