riscV/SelectOpproof.v
@@ -875,7 +875,11 @@ Theorem eval_select:
      eval_expr ge sp e m le a v
   /\ Val.lessdef (Val.select (eval_condition cond vl m) v1 v2 ty) v.
 Proof.
-  unfold select; intros; discriminate.
+  unfold select; intros.
+  destruct (select_supported ty); try discriminate.
+  destruct (select_swap cond); inv H.
+- TrivialExists. simpl. rewrite eval_negate_condition. destruct (eval_condition cond vl m) as [[]|]; simpl; auto.
+- TrivialExists.
 Qed.
 
 Theorem eval_addressing:
